theories/Stlc/Triangular.v
@@ -28,7 +28,6 @@
 
 From Coq Require Import
   Classes.Morphisms
-(*   Program.Basics *)
   Relations.Relation_Definitions.
 From Em Require Import
   Context
@@ -42,8 +41,6 @@ Import World.notations.
 
 #[local] Set Implicit Arguments.
 
-(* #[local] Open Scope indexed_scope. *)
-
 Reserved Notation "w1 ⊒⁻ w2" (at level 80).
 
 Definition Later (A : TYPE) : TYPE :=
@@ -55,16 +52,6 @@ Definition Sooner (A : TYPE) : TYPE :=
   fun w => sigT (fun x => sigT (fun (xIn : x ∈ w) => A (w - x))).
 Definition SoonerTm (A : TYPE) : TYPE :=
   fun w => sigT (fun x => sigT (fun (xIn : x ∈ w) => Ṫy (w - x) * A (w - x)))%type.
-
-(* Module Sng. *)
-
-(*   Inductive Sng (w : World) : World -> Set := *)
-(*   | sng {x} (xIn : x ∈ w) (t : Ṫy (w - x)) : Sng w (w - x). *)
-
-(*   #[export] Instance lk_sng : Lk Sng := *)
-(*     fun w0 w1 r => match r with sng xIn t => thickIn xIn t end. *)
-
-(* End Sng. *)
 
 Module Tri.
 
@@ -118,52 +105,6 @@ Module Tri.
       | cons x t ζ1 => fun ζ2 => cons x t (trans ζ1 ζ2)
       end.
 
-  (* Definition Raw_case [w] (P : forall w', w ⊒⁻ w' -> Type) *)
-  (*   (p_refl : P w Worlds.refl) *)
-  (*   (p_cons : forall w' x (xIn : x ∈ w) t r, P w' (thick x t ⊙ r)) *)
-  (*   {w'} (r : w ⊒⁻ w') : P w' r := *)
-  (*   match r with *)
-  (*   | refl       => p_refl *)
-  (*   | cons x t r => p_cons _ x _ t r *)
-  (*   end. *)
-
-  (* Definition Raw_rect (P : forall w w', Tri w w' -> Type) *)
-  (*   (p_refl : forall w : World, P w w Worlds.refl) *)
-  (*   (p_cons : forall w w' x (xIn : x ∈ w) t r, *)
-  (*       P (w - x) w' r -> P w w' (thick x t ⊙ r)) : *)
-  (*   forall w w' (r : w ⊒⁻ w'), P w w' r := *)
-  (*   fix rect w w' (r : w ⊒⁻ w') {struct r} : P w w' r := *)
-  (*     Raw_case (P w) (p_refl w) *)
-  (*       (fun _ x _ t r' => *)
-  (*          p_cons _ _ x _ t r' (rect _ _ r')) r. *)
-  (* Definition Raw_ind (P : forall w w', Tri w w' -> Prop) := Raw_rect P. *)
-  (* Definition Raw_rec (P : forall w w', Tri w w' -> Set) := Raw_rect P. *)
-
-  (* Definition Raw_sind (P : forall w w' : World, Raw w w' -> Type) *)
-  (*   (p_refl : forall w : World, P w w Worlds.refl) *)
-  (*   (p_cons : forall w w' x (xIn : x ∈ w) t r, *)
-  (*       P (w - x) w' r -> P w w' (thick x t ⊙ r)) := *)
-  (*   fix sind {w w'} (r : w ⊒⁻ w') {struct r} : P w w' r := *)
-  (*     match r with *)
-  (*     | refl => p_refl w *)
-  (*     | cons x t r => p_cons _ _ x _ t r (sind r) *)
-  (*     end. *)
-
-  (* Inductive onsubterms (P : forall w w', Raw w w' -> Type) {w} : *)
-  (*   forall w', w ⊒⁻ w' -> Type := *)
-  (* | on_refl : onsubterms P refl *)
-  (* | on_cons {x} (xIn : x ∈ w) (t : Ṫy (w - x)) {w'} (r : Tri (w - x) w') : *)
-  (*   P (w - x) w' r -> onsubterms P (cons x t r). *)
-  (* Arguments on_refl {P w}. *)
-  (* Arguments on_cons {P w} x {xIn} t {w' r} _. *)
-
-  (* Definition Tri_löb (P : forall w w', Raw w w' -> Type) *)
-  (*   (step : forall w w' r, onsubterms P r -> P w w' r) : *)
-  (*   forall w w' r, P w w' r := *)
-  (*   fix löb w w' (r : w ⊒⁻ w') {struct r} : P w w' r := *)
-  (*     Raw_case (P w) (step w w Worlds.refl on_refl) *)
-  (*       (fun w' x xIn t r => step w w' (thick x t ⊙ r) (on_cons x t (löb (w - x) w' r))) r. *)
-
   Module Import notations.
     Notation "▷ A" := (Later A) (at level 9, right associativity).
     Notation "▶ A" := (LaterTm A) (at level 9, right associativity).
@@ -180,8 +121,6 @@ Module Tri.
       | Tri.cons x t ζ' => la x _ t _ ζ'
       end.
 
-  (* Arguments Raw_ind (P p_refl p_cons)%function_scope (w w')%ctx_scope r. *)
-  (* Check @Raw_ind. *)
   #[export] Instance refltrans_tri : ReflTrans Tri.
   Proof.
     constructor.
@@ -189,97 +128,6 @@ Module Tri.
     - induction r; cbn; [|rewrite IHr]; easy.
     - induction r1; cbn; congruence.
   Qed.
-
-  (* #[export] Instance InstTri : forall w, Inst (Tri w) (Assignment w) := *)
-  (*   fix insttri {w0 w1} (r : Tri w0 w1) := *)
-  (*     match r with *)
-  (*     | Tri.refl => fun ι => ι *)
-  (*     | @Tri.cons _ w' x xIn t r => *)
-  (*         fun ι => *)
-  (*           let ι' := inst (Inst := @insttri _) r ι in *)
-  (*           env.insert xIn ι' (inst t ι') *)
-  (*     end. *)
-
-  (* #[export] Instance instrefl_tri : InstRefl Tri := *)
-  (*   fun _ _ => eq_refl. *)
-
-  (* Definition geq {w0 w1} (ζ1 : w0 ⊒⁻ w1) [w2] (ζ2 : w0 ⊒⁻ w2) : Prop := *)
-  (*   exists ζ12 : w1 ⊒⁻ w2, ζ2 = ζ1 ⊙ ζ12. *)
-  (* Notation "ζ1 ≽ ζ2" := (geq ζ1 ζ2) (at level 80). *)
-
-  (* Lemma geq_refl {w1 w2} (ζ : w1 ⊒⁻ w2) : ζ ≽ ζ. *)
-  (* Proof. exists refl. symmetry. apply trans_refl. Qed. *)
-
-  (* Lemma geq_trans {w0 w1 w2 w3} (ζ1 : w0 ⊒⁻ w1) (ζ2 : w0 ⊒⁻ w2) (ζ3 : w0 ⊒⁻ w3) : *)
-  (*   ζ1 ≽ ζ2 -> ζ2 ≽ ζ3 -> ζ1 ≽ ζ3. *)
-  (* Proof. *)
-  (*   intros [ζ12 H12] [ζ23 H23]. exists (ζ12 ⊙ ζ23). *)
-  (*   rewrite H23, H12. apply trans_assoc. *)
-  (* Qed. *)
-
-  (* Lemma geq_precom {w0 w1 w2 w3} (ζ1 : w0 ⊒⁻ w1) (ζ2 : w1 ⊒⁻ w2) (ζ3 : w1 ⊒⁻ w3) : *)
-  (*   ζ2 ≽ ζ3 -> ζ1 ⊙ ζ2 ≽ ζ1 ⊙ ζ3. *)
-  (* Proof. intros [ζ23 ->]. exists ζ23. symmetry. apply trans_assoc. Qed. *)
-
-  (* Lemma geq_max {w1 w2} (ζ : w1 ⊒⁻ w2) : refl ≽ ζ. *)
-  (* Proof. exists ζ. reflexivity. Qed. *)
-
-  (* Lemma geq_extend {w0 w1 w2} (ζ1 : w0 ⊒⁻ w1) (ζ2 : w1 ⊒⁻ w2) : ζ1 ≽ ζ1 ⊙ ζ2. *)
-  (* Proof. now exists ζ2. Qed. *)
-
-  (* Definition geqb1 [w0 z] (zIn : z ∈ w0) (tz : Ṫy (w0 - z)) [w1] (ζ : w0 ⊒⁻ w1) : *)
-  (*   option (w0 - z ⊒⁻ w1). *)
-  (* Proof. *)
-  (*   rename w1 into wend. *)
-  (*   induction ζ. *)
-  (*   + apply None. *)
-  (*   + rename w' into wend. rename t into tx. *)
-  (*     destruct (occurs_check_view xIn zIn). *)
-  (*     * refine (if Ty_eqdec tx tz then Some ζ else None). *)
-  (*     * rename y into z. rename yIn into zIn. *)
-  (*       specialize (IHζ zIn). *)
-  (*       Check (thick (thin _ tz) _ tx). *)
-  (* Admitted. *)
-
-  (* Fixpoint geqb (w0 w1 : World) (ζ1 : w0 ⊒⁻ w1) {w2} (ζ2 : w0 ⊒⁻ w2) {struct ζ1} : *)
-  (*   option (w1 ⊒⁻ w2) := *)
-  (*   match ζ1 with *)
-  (*   | refl => Some ζ2 *)
-  (*   | cons x t__X ζ1' => *)
-  (*       option.bind (geqb1 _ t__X ζ2) (geqb ζ1') *)
-  (*   end. *)
-
-  (* Lemma geqb_spec {w0 w1} (ζ1 : w0 ⊒⁻ w1) : *)
-  (*   forall [w2] (ζ2 : w0 ⊒ˢ w2), *)
-  (*     Bool.reflect (triangular ζ1 ≽ ζ2) (ζ1 ≽? ζ2). *)
-  (* Proof. *)
-  (*   induction ζ1; cbn [geqb triangular]; intros w2 ζ2. *)
-  (*   - constructor. apply geq_max. *)
-  (*   - destruct Ty_eqdec. *)
-  (*     + destruct (IHζ1 _ (thin xIn ⊙ˢ ζ2)); constructor; clear IHζ1. *)
-  (*       * destruct g as [ζ2']. exists ζ2'. *)
-  (*         rewrite comp_assoc. rewrite <- H. clear - e. *)
-  (*         apply env.lookup_extensional. *)
-  (*         intros y yIn. *)
-  (*         rewrite lookup_comp. *)
-  (*         rewrite lookup_thick. unfold thickIn. *)
-  (*         destruct (occurs_check_view xIn yIn). apply e. *)
-  (*         cbn. rewrite lookup_comp. unfold thin. *)
-  (*         now rewrite env.lookup_tabulate. *)
-  (*       * intros [ζ2' ->]. apply n. clear n. exists ζ2'. *)
-  (*         rewrite <- ?comp_assoc. *)
-  (*         rewrite comp_thin_thick. *)
-  (*         rewrite comp_id_left. *)
-  (*         reflexivity. *)
-  (*     + constructor. intros [ζ2' ->]. apply n. clear n. *)
-  (*       rewrite <- ?comp_assoc. *)
-  (*       rewrite comp_thin_thick. *)
-  (*       rewrite comp_id_left. *)
-  (*       cbn. rewrite ?lookup_comp, lookup_thick. *)
-  (*       unfold thickIn. rewrite occurs_check_view_refl. *)
-  (*       now rewrite subst_comp. *)
-  (* Qed. *)
-
 
   #[export] Instance lkrefl_tri : LkRefl Tri.
   Proof. intros w α αIn. reflexivity. Qed.
@@ -326,28 +174,8 @@ Module Tri.
     now rewrite persist_outer_trans, persist_outer_persist.
   Qed.
 
-  (* Corollary persist_bool {w0 w1} (r : Tri w0 w1) : *)
-  (*   persist _ Ty_bool _ r = Ty_bool. *)
-  (* Proof. apply (persist_fix r). Qed. *)
-
-  (* Corollary persist_func {w0 w1} (r : Tri w0 w1) (t1 t2 : Ṫy w0) : *)
-  (*   persist _ (Ty_func t1 t2) _ r = Ty_func (persist _ t1 _ r) (persist _ t2 _ r). *)
-  (* Proof. apply (persist_fix r). Qed. *)
-
-
-  (* #[export] Instance persist_preorder_tri : PersistPreOrder Tri Ty. *)
-  (* Proof. *)
-  (*   constructor. *)
-  (*   - reflexivity. *)
-  (*   - intros w0 t w1 w2 ζ1 ζ2. *)
-  (*     induction ζ1; cbn; intros *. *)
-  (*     + reflexivity. *)
-  (*     + rewrite persist_persist_inner. *)
-  (*       now apply proper_persist_inner. *)
-  (* Qed. *)
-
-  (* #[export] Instance inst_thick : InstThick Tri. *)
-  (* Proof. easy. Qed. *)
+  #[export] Instance lkthick_tri : LkThick Tri.
+  Proof. easy. Qed.
 
 End Tri.
 Export Tri (Tri).
